\section{Solve}
\subsubsection{ABS-Equation-System}

As a last step we bring the function in the form of a linear equation system.

\begin{flalign*}
	\begin{pmatrix}
		\Delta z \\
		\Delta y
	\end{pmatrix}
	= 
	\begin{pmatrix}
		a \\
		b
	\end{pmatrix}
	+
	\begin{pmatrix}
		Z & L \\
		J & Y 
	\end{pmatrix}
	\times
	\begin{pmatrix}
		\Delta x \\
		|\Delta z|
	\end{pmatrix}
\end{flalign*}
We assume:
\begin{flalign*}
	\Delta y = 0
\end{flalign*}
otherwise use
\begin{flalign*}
	b' = b - \Delta y
\end{flalign*}

\begin{flalign*}
	\Delta y &= b + J \Delta x + Y |\Delta z| \\
	0 &= b + J \Delta x + Y |\Delta z| \\
	- b - Y |\Delta z| &= J \Delta x \\
	b - Y |\Delta z| &= J \Delta x (-1) \\
	J^{-1}(b - Y |\Delta z|) &= - \Delta x \\
	\Delta x = - J^{-1}(b - Y |\Delta z|)
\end{flalign*}

\begin{flalign*}
	\Delta z &= a + Z \Delta x + L |\Delta z| \\
	&= a + Z \Big( - J^{-1}(b - Y |\Delta z|) \Big) +  L |\Delta z| \\
	&= a + Z \Big( -J^{-1}b + J^{-1}Y|\Delta z| \Big) +  L |\Delta z| \\
	&= a - ZJ^{-1}b + Z J^{-1}Y|\Delta z| +  L |\Delta z| \\
	&= a - ZJ^{-1}b + (Z J^{-1}Y + L)|\Delta z|
\end{flalign*}
\begin{flalign*}
\Delta z &= a - ZJ^{-1}b + (Z J^{-1}Y + L)|\Delta z| \\
\Delta z &= c + S|\Delta z| \\
c		 &= a - ZJ^{-1}b \\
S		 &= (Z J^{-1}Y + L)
\end{flalign*}

\subsection{Useless}
\begin{flalign*}
	a' = a - \Delta z
\end{flalign*}
\begin{flalign*}
	0 &= a' - ZJ^{-1}b + (Z J^{-1}Y + L)|\Delta z| \\
	- a' + ZJ^{-1}b &= (Z J^{-1}Y + L)|\Delta z| \\
	(Z J^{-1}Y + L)^{-1} (-a' + ZJ^{-1}b) &= |\Delta z|
\end{flalign*}